prove Lock

ironfleet/src/Dafny/Distributed/LockProof/p_s_lemma.i.dfy
@@ -4,7 +4,7 @@ include "../Services/Lock/AbstractService.s.dfy"
 include "p_s_correspondence.s.dfy"
 
 
-module P_S_Lemma {
+abstract module P_S_Lemma {
 import opened DistributedSystem_i
 import opened Protocol_Node_i
 import opened AbstractServiceLock_s
@@ -74,30 +74,27 @@ predicate LS_GLS_Correspondence(packets:set<LockPacket>, gls:GLS_State, config:C
             && p.src == gls.history[epoch-1]
 }
 
-predicate LS_GLS_Transfer_Correspondence(packets:set<LockPacket>, gls:GLS_State, config:Config) {
-    
-    forall p ::
-           p in packets
-        && p.src in config
-        && p.dst in config
-        && p.msg.Transfer?
-        ==> var epoch := p.msg.transfer_epoch;
-                0 < epoch <= |gls.history|
-            && p.src == gls.history[epoch-1]
-}
-
 predicate Transfer_Epoch_In_History(gls:GLS_State, config:Config) {
     forall p ::
            p in gls.ls.environment.sentPackets
         && p.msg.Transfer?
         && p.src in config
-       ==> 2 <= p.msg.transfer_epoch <= |gls.history|
+       ==> var epoch := p.msg.transfer_epoch;
+           2 <= epoch <= |gls.history|
+        && gls.history[epoch-1] == p.dst
 }
 
 predicate Hold_Epoch(gls:GLS_State) {
     forall s :: s in gls.ls.servers
              && gls.ls.servers[s].held
             ==> gls.ls.servers[s].epoch == |gls.history|
+}
+
+predicate Hold_History(gls:GLS_State) {
+    forall s :: s in gls.ls.servers
+             && gls.ls.servers[s].held
+             && |gls.history| > 0
+            ==> s == gls.history[|gls.history|-1]
 }
 
 predicate Unique_Hold(s:LS_State) {
@@ -109,54 +106,79 @@ predicate Unique_Hold(s:LS_State) {
        ==> x == y 
 }
 
+predicate Less_Than_One_Hold(gls:GLS_State) {
+
+       (|gls.history| > 0 && forall s ::   
+                                    s in gls.ls.servers
+                                ==> (s == gls.history[|gls.history|-1] <==> gls.ls.servers[s].held))
+    || (|gls.history| > 1 && exists p :: 
+                                    p in gls.ls.environment.sentPackets
+                                 && p.msg.Transfer?
+                                 && p.dst == gls.history[|gls.history|-1]
+                                 && p.src == gls.history[|gls.history|-2]
+                          && forall s :: s in gls.ls.servers ==> !gls.ls.servers[s].held)
+
+}
+
+predicate Epoch_History(gls:GLS_State) {
+
+    forall s, e ::
+           s in gls.ls.servers
+        && 0 <= e < |gls.history|
+        && gls.history[e] == s
+        && (e != |gls.history| - 1 || gls.ls.servers[s].held)
+       ==> gls.ls.servers[s].epoch >= e+1
+}
+
 lemma History_Len(gls:seq<GLS_State>, config:Config)
 requires |gls| > 0
 requires GLS_Init(gls[0], config)
 requires forall i :: 0 <= i < |gls|-1 ==> GLS_Next(gls[i], gls[i+1]) || gls[i] == gls[i+1]
 ensures forall i :: 0 <= i < |gls| ==> |gls[i].history| >= 1
-{}
-
-lemma At_Most_One_Hold(config:Config, ls:seq<LS_State>)
-requires |ls| > 0
-requires LS_Init(ls[0], config)
-requires forall i :: 0 <= i < |ls|-1 ==> LS_Next(ls[i], ls[i+1]) || ls[i] == ls[i+1]
-ensures forall i :: 0 <= i < |ls| ==> Unique_Hold(ls[i]);
 {
-    assert Unique_Hold(ls[0]);
+    assert |gls[0].history| >= 1;
+
     var k := 1;
-    while (k < |ls|)
-    invariant 1 <= k <= |ls|
-    invariant forall i :: 0 <= i < k ==> Unique_Hold(ls[i])
+    while (k < |gls|) 
+    invariant 1 <= k <= |gls|
+    invariant forall i :: 0 <= i < k ==> |gls[i].history| >= 1
     {
-        var kk := k-1;
-
-        if (LS_Next(ls[kk], ls[kk+1])
-         && ls[kk].environment.nextStep.LEnvStepHostIos?
-         && ls[kk].environment.nextStep.actor in ls[kk].servers) {
-            var s := ls[kk];
-            var s' := ls[kk+1];
-            var id := s.environment.nextStep.actor;
-            var ios := s.environment.nextStep.ios;
-            assert s'.servers == s.servers[id := s'.servers[id]];
-            
-            forall x | x in s'.servers 
-            ensures !s'.servers[x].held
-            {
-                if (x != id) {
-                    assert s'.servers[x].held == s.servers[x] == false;
-                } else {
-                    assert !s'.servers[x].held;
-                }
-            }
-
-            assert Unique_Hold(ls[kk+1]);
-        } 
-        
+        var kk := k - 1;
+        if (GLS_Next(gls[k-1], gls[k])) {
+            assert |gls[k].history| >= 1;
+        } else {
+            assert gls[kk] == gls[kk+1];
+            assert |gls[k].history| >= 1;
+        }
         k := k + 1;
     }
 }
 
+lemma UniqueHold(s:GLS_State)
+requires Hold_History(s)
+requires |s.history| > 0
+ensures forall i, j :: 
+               i in s.ls.servers
+            && j in s.ls.servers
+            && s.ls.servers[i].held
+            && s.ls.servers[j].held
+           ==> i == j
+{
+    forall i, j |
+           i in s.ls.servers
+        && j in s.ls.servers
+        && s.ls.servers[i].held
+        && s.ls.servers[j].held
+    ensures i == j
+    {
+        assert i == s.history[|s.history|-1];
+        assert j == s.history[|s.history|-1];
+    }
+}
+
 lemma Hold_Epoch_Next(s:GLS_State, s':GLS_State)
+requires |s.history| > 0
+requires |s'.history| > 0
 requires GLS_Next(s, s')
 requires s.ls.environment.nextStep.LEnvStepHostIos?
 requires s.ls.environment.nextStep.actor in s.ls.servers
@@ -164,7 +186,12 @@ requires NodeGrant(s.ls.servers[s.ls.environment.nextStep.actor], s'.ls.servers[
 requires s.ls.servers[s.ls.environment.nextStep.actor].held
 requires s.ls.servers[s.ls.environment.nextStep.actor].epoch < 0xFFFF_FFFF_FFFF_FFFF
 requires Hold_Epoch(s)
+requires Hold_History(s)
+requires Epoch_History(s)
+requires Less_Than_One_Hold(s)
 ensures Hold_Epoch(s')
+ensures Epoch_History(s')
+ensures Less_Than_One_Hold(s')
 {
     forall ss |
            ss in s'.ls.servers
@@ -180,6 +207,32 @@ ensures Hold_Epoch(s')
         }
     }
 
+    forall ss, e | 
+           ss in s'.ls.servers
+        && 0 <= e < |s'.history|
+        && s'.history[e] == ss
+        && (e != |s'.history|-1 || s'.ls.servers[ss].held)
+    ensures s'.ls.servers[ss].epoch >= e+1
+    {
+        assert |s'.history| == |s.history| + 1;
+        if (e < |s.history|) {
+            assert s'.ls.servers[ss].epoch >= e+1;
+        }
+    }
+
+    var id := s.ls.environment.nextStep.actor;
+    var ios := s.ls.environment.nextStep.ios;
+    assert |ios| == 1;
+    assert ios[0].LIoOpSend?;
+    assert ios[0].s.msg.Transfer?;
+    assert IsValidLIoOp(ios[0], id, s.ls.environment);
+    assert ios[0].s.src == id;
+    assert |s.history| > 0;
+    assert |s'.history| > 1;
+    assert id == s.history[|s.history|-1] == s'.history[|s'.history|-2];
+    assert ios[0].s.dst == s'.history[|s'.history|-1];
+    assert Less_Than_One_Hold(s');
+
 }
 
 
@@ -194,6 +247,7 @@ requires forall j :: j in s.ls.servers ==> s.ls.servers[j].config == config
 requires forall j :: j in config <==> j in s.ls.servers
 requires Transfer_Epoch_In_History(s, config)
 requires s.ls.environment.nextStep.ios[0].s.msg.transfer_epoch == |s'.history|;
+requires s'.history == s.history + [s.ls.servers[s.ls.environment.nextStep.actor].config[(s.ls.servers[s.ls.environment.nextStep.actor].my_index + 1) % |s.ls.servers[s.ls.environment.nextStep.actor].config|]];
 requires |s'.history| > 1
 ensures Transfer_Epoch_In_History(s', config)
 {
@@ -213,10 +267,13 @@ ensures Transfer_Epoch_In_History(s', config)
         && p.msg.Transfer?
         && p.src in config
     ensures 2 <= p.msg.transfer_epoch <= |s'.history|
+    ensures p.dst == s'.history[p.msg.transfer_epoch-1]
     {
+        var epoch := p.msg.transfer_epoch;
         if (p == ios[0].s) {
-            assert p.msg.transfer_epoch == |s'.history|;
-            assert 2 <= p.msg.transfer_epoch <= |s'.history|;
+            assert epoch == |s'.history|;
+            assert 2 <= epoch <= |s'.history|;
+            assert p.dst == s.ls.servers[s.ls.environment.nextStep.actor].config[(s.ls.servers[s.ls.environment.nextStep.actor].my_index + 1) % |s.ls.servers[s.ls.environment.nextStep.actor].config|];
         }
     }
 }
@@ -240,9 +297,15 @@ requires forall j :: j in s'.ls.servers ==> s'.ls.servers[j].config == config
 requires Transfer_Epoch_In_History(s, config);
 requires LS_GLS_Correspondence(s.ls.environment.sentPackets, s, config)
 requires Hold_Epoch(s)
+requires Hold_History(s)
+requires Less_Than_One_Hold(s)
+requires Epoch_History(s)
 ensures LS_GLS_Correspondence(s'.ls.environment.sentPackets, s', config)
 ensures Hold_Epoch(s')
 ensures Transfer_Epoch_In_History(s', config)
+ensures Hold_History(s')
+ensures Less_Than_One_Hold(s')
+ensures Epoch_History(s')
 {
     var id := s.ls.environment.nextStep.actor;
     var ios := s.ls.environment.nextStep.ios;
@@ -260,13 +323,38 @@ ensures Transfer_Epoch_In_History(s', config)
                && p.msg.Transfer?
                && p.src in config
                && p.msg.transfer_epoch == ios[1].s.msg.locked_epoch;
-    
 
+    assert LEnvironment_Next(s.ls.environment, s'.ls.environment);
+    assert IsValidLIoOp(ios[0], id, s.ls.environment);
+    assert id == ios[0].r.dst;
+    assert ios[0].r.msg.transfer_epoch >= s.ls.servers[id].epoch;
+
+    var epoch := ios[0].r.msg.transfer_epoch;
+    if (ios[0].r.msg.transfer_epoch < |s.history|) {
+        assert s.history[epoch-1] == ios[0].r.dst == id;
+        assert s.ls.servers[id].epoch >= epoch;
+    }
+
+
+    assert ios[0].r.msg.transfer_epoch == |s.history|;
+    assert ios[0].r.dst == s.history[|s.history|-1];
+    assert id == s.history[|s.history|-1];
+    assert Less_Than_One_Hold(s');
+    assert Hold_History(s');
+
+    assert Hold_Epoch(s);
+    assert s'.ls.servers[id].epoch == ios[1].s.msg.locked_epoch;
+    assert s'.ls.servers[id].epoch == ios[0].r.msg.transfer_epoch;
+    
+    
+    assert id == s.history[|s.history|-1];
+    assert ios[0].r.msg.transfer_epoch > s.ls.servers[id].epoch;
+    assert ios[0].r.msg.transfer_epoch == |s.history|;
+    assert ios[0].r.msg.transfer_epoch == |s'.history|;
+    assert Hold_Epoch(s'); 
 
     assert 2 <= ios[1].s.msg.locked_epoch <= |s'.history|; 
-    assert s'.history[ios[1].s.msg.locked_epoch-1] == ios[1].s.src; //(3)
-
-
+    assert s'.history[ios[1].s.msg.locked_epoch-1] == ios[1].s.src;
 
     assert LS_GLS_Correspondence(s.ls.environment.sentPackets, s', config);
     assert forall p ::
@@ -278,8 +366,8 @@ ensures Transfer_Epoch_In_History(s', config)
          && p.src == s'.history[p.msg.locked_epoch-1];
     
     assert LS_GLS_Correspondence(s'.ls.environment.sentPackets, s', config);
-    assert Hold_Epoch(s'); 
 
+    assert Epoch_History(s');
 
 }
 
