ironfleet/src/Dafny/Distributed/LockProof/Main.i.dfy
@@ -1,0 +1,464 @@
+include "../Common/Framework/Main.s.dfy"
+include "../Protocol/Lock/RefinementProof/DistributedSystem.i.dfy"
+include "../Services/Lock/AbstractService.s.dfy"
+include "../Impl/Lock/Host.i.dfy"
+include "../Impl/lock/Node.i.dfy"
+include "../Impl/Lock/NodeImpl.i.dfy"
+include "../Common/Collections/Seqs.s.dfy"
+include "../Common/Framework/DistributedSystem.s.dfy"
+include "proof.i.dfy"
+
+abstract module Main_i refines Main_s {
+    import opened DS_s = DistributedSystem_i  
+    import opened LockProof
+    import opened AS_s = AbstractServiceLock_s
+    import opened Host_i 
+
+    type RealMsg = seq<byte>;
+    // function ConstructLockMessage(msg:RealMsg) : LockMessage
+    // {
+    //     AbstractifyCMessage(DemarshallData(msg))
+    // }
+
+    // function AbstractifyUdpPacket(p:LPacket<EndPoint, RealMsg>) : LPacket<EndPoint, LockMessage>
+    // {
+    //     LPacket(p.src, p.dst, ConstructLockMessage(p.msg))
+    // }
+
+    function ConstructSentPackets(ps:set<LPacket<EndPoint, RealMsg>>) : set<LPacket<EndPoint, LockMessage>>
+    {
+        set p | p in ps :: AbstractifyUdpPacket(p)
+    }
+
+    function ConstructNextStep(nextStep:LEnvStep<EndPoint, RealMsg>) : LEnvStep<EndPoint, LockMessage> 
+    {
+        match nextStep {
+            case LEnvStepHostIos(actor, ios) => LEnvStepHostIos(actor, AbstractifyRawLogToIos(ios))
+            case LEnvStepDeliverPacket(p) => LEnvStepDeliverPacket(AbstractifyUdpPacket(p))
+            case LEnvStepAdvanceTime => LEnvStepAdvanceTime()
+            case LEnvStepStutter => LEnvStepStutter()
+        }
+    }
+
+    function ConstructLEnv(env:LEnvironment<EndPoint, RealMsg>) : LockEnvironment
+    {
+        var step := ConstructNextStep(env.nextStep);
+
+        LEnvironment(env.time, ConstructSentPackets(env.sentPackets), map [], step)
+    }
+
+    function ConstructServers(servers:map<EndPoint, Host_i.HostState>) : map<EndPoint, Node>
+    {
+        map i | i in servers :: servers[i].node
+    }
+
+    function Construct_LS_State(ds:DS_State) : LS_State
+    {
+        var environment := ConstructLEnv(ds.environment);
+        var servers := ConstructServers(ds.servers);
+        LS_State(environment, servers)
+    }
+
+    lemma ValidLEnvTransfer(de:LEnvironment<EndPoint, RealMsg>)
+    requires IsValidLEnvStep(de, de.nextStep)
+    ensures IsValidLEnvStep(ConstructLEnv(de), ConstructLEnv(de).nextStep)
+    {
+        var le := ConstructLEnv(de);
+        var step := le.nextStep;
+        if (step.LEnvStepHostIos?) {
+            var actor := step.actor;
+            var ios := step.ios;
+            assert de.nextStep.LEnvStepHostIos?;
+            var dactor := de.nextStep.actor;
+            var dios := de.nextStep.ios;
+            assert actor == dactor;
+            forall i |
+                   0 <= i < |ios|
+            ensures IsValidLIoOp(ios[i], actor, le)
+            {   
+                assert ios[i] == AstractifyUdpEventToLockIo(dios[i]);
+                match ios[i] {
+                    case LIoOpSend(s) => {
+                        assert dios[i].LIoOpSend?;
+                        assert s.src == dios[i].s.src;
+                        assert IsValidLIoOp(dios[i], dactor, de);
+                        assert dios[i].s.src == dactor;
+                        assert s.src == actor;
+                    }
+                    case LIoOpReceive(r) => {
+                        assert dios[i].LIoOpReceive?;
+                        assert r.dst == dios[i].r.dst;
+                        assert IsValidLIoOp(dios[i], dactor, de);
+                        assert dios[i].r.dst == dactor;
+                        assert r.dst == actor;
+                    }
+                    case LIoOpTimeoutReceive => assert true;
+                    case LIoOpReadClock(t) => assert true;
+                }
+                assert IsValidLIoOp(ios[i], actor, le);
+            }
+        } 
+    }
+
+
+    lemma DS_Next_Implies_LEnv_Next(ds:DS_State, ds':DS_State)
+    requires DS_Next(ds, ds')
+    ensures LEnvironment_Next(Construct_LS_State(ds).environment, Construct_LS_State(ds').environment)
+    {
+        var ls := Construct_LS_State(ds);
+        var ls':= Construct_LS_State(ds');
+        assert IsValidLEnvStep(ds.environment, ds.environment.nextStep);
+        ValidLEnvTransfer(ds.environment);
+        assert IsValidLEnvStep(ls.environment, ls.environment.nextStep);
+        match ls.environment.nextStep {
+            case LEnvStepHostIos(actor, ios) => 
+                assert LEnvironment_PerformIos(ds.environment, 
+                                               ds'.environment, 
+                                               ds.environment.nextStep.actor, 
+                                               ds.environment.nextStep.ios);
+
+                var de := ds.environment;
+                var de':= ds'.environment;
+                var le := ls.environment;
+                var le':= ls'.environment;
+                assert de.nextStep.LEnvStepHostIos?;
+                var dactor := de.nextStep.actor;
+                var dios := de.nextStep.ios;
+
+
+                assert de'.sentPackets == de.sentPackets + (set io | io in dios && io.LIoOpSend? :: io.s);
+
+                var dsent := set io | io in dios && io.LIoOpSend? :: io.s;
+                var lsent := set io | io in ios && io.LIoOpSend? :: io.s;
+                assert ios == AbstractifyRawLogToIos(dios);
+
+                forall i |
+                       0 <= i < |ios|
+                ensures ios[i].LIoOpSend? == dios[i].LIoOpSend?
+                ensures ios[i].LIoOpSend? ==> (ios[i].s == AbstractifyUdpPacket(dios[i].s))
+                {}
+
+                assert lsent == ConstructSentPackets(dsent);
+                assert le'.sentPackets == le.sentPackets + (set io | io in ios && io.LIoOpSend? :: io.s);
+                forall i |
+                       0 <= i < |ios|
+                    && ios[i].LIoOpReceive?
+                ensures ios[i].r in le.sentPackets
+                {
+                    assert dios[i].r in de.sentPackets;
+                    assert le.sentPackets == set p | p in de.sentPackets :: AbstractifyUdpPacket(p);
+                    assert ios[i] == AstractifyUdpEventToLockIo(dios[i]);
+                    assert ios[i].r == AbstractifyUdpPacket(dios[i].r);
+                    assert ios[i].r in le.sentPackets;
+                }
+
+                assert LEnvironment_PerformIos(ls.environment, ls'.environment, actor, ios);
+            case LEnvStepDeliverPacket(p) => 
+                assert LEnvironment_Stutter(ls.environment, ls'.environment);
+            case LEnvStepAdvanceTime => 
+                assert LEnvironment_AdvanceTime(ls.environment, ls'.environment);
+            case LEnvStepStutter => 
+                assert LEnvironment_Stutter(ls.environment, ls'.environment);
+        }
+    }
+
+    lemma DS_Next_Implies_LS_Next(ds:DS_State, ds':DS_State)
+    requires DS_Next(ds, ds')
+    ensures LS_Next(Construct_LS_State(ds), Construct_LS_State(ds'))
+    {
+        var ls := Construct_LS_State(ds);
+        var ls':= Construct_LS_State(ds');
+
+        DS_Next_Implies_LEnv_Next(ds, ds');
+        assert LEnvironment_Next(ls.environment, ls'.environment);
+    }
+
+
+    lemma BoundedEpoch(lmsg:LockMessage, dmsg:RealMsg, epoch:int) 
+    requires MarshallLockMsg(epoch) == dmsg;
+    requires lmsg == AbstractifyCMessage(DemarshallData(dmsg))
+    requires Demarshallable(dmsg, CMessageGrammar())
+    ensures 0 <= epoch < 0x1_0000_0000_0000_0000
+    {
+        // var g := CMessageGrammar();
+        // var pv := parse_Val(dmsg, g);
+        // assert !parse_Val(dmsg, g).0.None?;
+        reveal_parse_Val();
+        // var (v, rest) := parse_Val(dmsg, g);
+
+    }
+
+
+    lemma parse_Val_to_parse_Case(parsed:(Option<V>, seq<byte>), dmsg:RealMsg, grammar:G)
+    requires |dmsg| < 0x1_0000_0000_0000_0000
+    requires ValidGrammar(grammar)
+    requires parsed == parse_Val(dmsg, grammar)
+    requires grammar.GTaggedUnion?;
+    ensures parsed == parse_Case(dmsg, grammar.cases)
+    {
+        reveal_parse_Val();
+    }
+
+    lemma IntToBytesParsedBack(rest:seq<byte>, vv:Option<V>, rest2:seq<byte>, epoch:int)
+    requires 0 <= epoch < 0x1_0000_0000_0000_0000
+    requires rest == Uint64ToBytes(uint64(epoch))
+    requires (vv, rest2) == parse_Uint64(rest)
+    ensures int(vv.v.u) == epoch
+    {
+        assert rest == Uint64ToSeqByte(uint64(epoch));
+        assert rest == BEUintToSeqByte(epoch, 8);
+        lemma_2toX();
+        calc {
+            power2(8*8);
+        }
+        assert 0 <= epoch < power2(8*8);
+        lemma_BEUintToSeqByte_invertability(rest, epoch, 8);
+        assert BEByteSeqToInt(rest) == epoch;
+        assert SeqByteToUint64(rest) == uint64(epoch);
+    }
+
+
+    lemma DemarshallMessageResultsInCorrectEpoch(dmsg:RealMsg, val:V, g:G, epoch:int, caseID:Option<V>, rest1:seq<byte>, vv:Option<V>, rest2:seq<byte>)
+    requires 0 <= epoch < 0x1_0000_0000_0000_0000
+    requires MarshallLockMsg(epoch) == dmsg
+    requires Demarshallable(dmsg, g)
+    requires g == CMessageGrammar()
+    requires g.GTaggedUnion?
+    requires val == DemarshallFunc(dmsg, g)
+    requires val.val.VUint64?
+    requires (caseID, rest1) == parse_Uint64(dmsg)
+    requires (vv, rest2) == parse_Uint64(rest1)
+    requires val.val == vv.v
+    ensures int(val.val.u) == epoch
+    {
+        // assert dmsg[8..] == rest1;
+        // assert dmsg == [0,0,0,0,0,0,0,1] + rest1;
+        assert rest1 == Uint64ToBytes(uint64(epoch));
+        // assert dmsg[8..] == Uint64ToBytes(uint64(epoch));
+
+        IntToBytesParsedBack(rest1, vv, rest2, epoch);
+        assert int(vv.v.u) == epoch;
+    }
+
+    lemma DemarshallMessageResultsInCLocked(dmsg:RealMsg, val:V, g:G, epoch:int)
+    requires 0 <= epoch < 0x1_0000_0000_0000_0000
+    requires MarshallLockMsg(epoch) == dmsg
+    requires Demarshallable(dmsg, g)
+    requires g == CMessageGrammar()
+    requires g.GTaggedUnion?
+    requires val == DemarshallFunc(dmsg, g)
+    ensures val.c == 1
+    ensures val.val.VUint64?
+    ensures int(val.val.u) == epoch
+    {
+        reveal_parse_Val();
+        assert val == parse_Case(dmsg, g.cases).0.v;
+
+
+        var (caseID, rest1) := parse_Uint64(dmsg);
+        assert !caseID.None?;
+        assert caseID.v.u < uint64(|g.cases|);
+        var (vv, rest2) := parse_Val(rest1, g.cases[caseID.v.u]);
+        assert !vv.None?;
+        assert val.c == caseID.v.u;
+        assert val.val == vv.v;
+        assert caseID.v.u == 1;
+        assert g.cases[caseID.v.u] == CMessageLockedGrammar();
+        assert vv.v.VUint64?;
+
+        DemarshallMessageResultsInCorrectEpoch(dmsg, val, g, epoch, caseID, rest1, vv, rest2);
+    }
+
+
+    lemma MarshallLockedMsg(lmsg:LockMessage, dmsg:RealMsg, epoch:int) 
+    requires MarshallLockMsg(epoch) == dmsg;
+    requires lmsg == AbstractifyCMessage(DemarshallData(dmsg))
+    requires Demarshallable(dmsg, CMessageGrammar())
+    ensures lmsg.Locked?
+    ensures lmsg.locked_epoch == epoch
+    {   
+
+        BoundedEpoch(lmsg, dmsg, epoch);
+        assert 0 <= epoch < 0x1_0000_0000_0000_0000;
+
+        // var cmsg := DemarshallData(dmsg);
+        // var val := DemarshallFunc(dmsg, CMessageGrammar());
+        var grammar := CMessageGrammar();
+        assert grammar.GTaggedUnion?;
+
+        var val := DemarshallFunc(dmsg, grammar);
+        DemarshallMessageResultsInCLocked(dmsg, val, grammar, epoch);
+        assert val.c == 1;
+        assert int(val.val.u) == epoch;
+
+    }
+
+
+    lemma ServiceCorrespondenceTransfer(ds:DS_State, ss:ServiceState)
+    requires Protocol_Service_Correspondence(
+                Construct_LS_State(ds).environment.sentPackets,
+                ss)
+    requires forall p :: 
+                    p in ds.environment.sentPackets 
+                 && p.src in ss.hosts
+                ==> Demarshallable(p.msg, CMessageGrammar())
+    ensures Service_Correspondence(ds.environment.sentPackets, ss)
+    {
+        var ps := ds.environment.sentPackets;
+        forall p, epoch |
+               p in ps
+            && p.src in ss.hosts
+            && p.dst in ss.hosts
+            && p.msg == MarshallLockMsg(epoch)
+        ensures 1 <= epoch <= |ss.history|
+        ensures p.src == ss.history[epoch-1]
+        {
+            var ls := Construct_LS_State(ds);
+            var lps:= ls.environment.sentPackets;
+            var lp := AbstractifyUdpPacket(p);
+            var c := DemarshallData(p.msg);
+            assert lp in lps;
+            assert Demarshallable(p.msg, CMessageGrammar());
+            MarshallLockedMsg(lp.msg, p.msg, epoch);
+            assert lp.msg.Locked?;
+            assert 1 <= lp.msg.locked_epoch <= |ss.history|;
+            assert epoch == lp.msg.locked_epoch;
+        }
+    }
+
+
+    lemma InitTransfer(ds:DS_State, config:ConcreteConfiguration)
+    requires DS_Init(ds, config)
+    ensures LS_Init(Construct_LS_State(ds), config)
+    {
+        var ls := Construct_LS_State(ds);
+        assert LEnvironment_Init(ls.environment);
+        assert |config| > 0;
+        assert SeqIsUnique(config);
+        assert forall e :: e in config <==> e in ls.servers;
+        forall index |
+               0 <= index < |config|
+        ensures NodeInit(ls.servers[config[index]], index, config)
+        {
+            assert mapdomain(ds.servers) == MapSeqToSet(config, x=>x);
+            assert config[index] in config;
+            assert forall xx :: xx in config <==> xx in MapSeqToSet(config, x=>x);
+            assert config[index] in MapSeqToSet(config, x=>x);
+            assert config[index] in ds.servers;
+            assert HostInit(ds.servers[config[index]], config, config[index]);
+            var host_state := ds.servers[config[index]];
+            assert config[host_state.node_impl.node.my_index] == config[index];
+            assert SeqIsUnique(config);
+            reveal_SeqIsUnique();
+            assert forall i, j :: 
+                   0 <= i < |config|
+                && 0 <= j < |config|
+                && config[i] == config[j]
+               ==> i == j;
+            assert host_state.node_impl.node.my_index == uint64(index);
+        }
+                    
+    }
+
+    predicate SentDemarshallable(ps:set<LPacket<EndPoint, RealMsg>>, config:ConcreteConfiguration)
+    {
+        forall p ::
+               p in ps
+            && p.src in config
+           ==> Demarshallable(p.msg, CMessageGrammar())
+    }
+
+
+    lemma Valid_Db_Implies_Demarshallable(db:seq<DS_State>, config:ConcreteConfiguration)
+    requires |db| > 0
+    requires DS_Init(db[0], config)
+    requires forall i :: 0 <= i < |db|-1 ==> DS_Next(db[i], db[i+1])
+    ensures forall i :: 0 <= i < |db| ==> SentDemarshallable(db[i].environment.sentPackets, config)
+    {
+        assert SentDemarshallable(db[0].environment.sentPackets, config);
+
+        var k := 1;
+        while (k < |db|)
+        invariant 0 <= k <= |db|
+        invariant forall i :: 0 <= i < k ==> SentDemarshallable(db[i].environment.sentPackets, config)
+        invariant forall i :: 0 <= i < k ==> forall j :: j in db[i].servers <==> j in config
+        {
+            var kk := k - 1;
+            assert DS_Next(db[kk], db[kk+1]);
+            assert forall i :: i in db[kk].servers <==> i in config;
+            if (db[kk].environment.nextStep.LEnvStepHostIos? 
+             && db[kk].environment.nextStep.actor in db[kk].servers) {
+                var id := db[kk].environment.nextStep.actor;
+                var ios := db[kk].environment.nextStep.ios;
+                assert HostNext(db[kk].servers[id], db[kk+1].servers[id], ios);
+                assert OnlySentMarshallableData(db[kk].environment.nextStep.ios);
+                assert SentDemarshallable(db[kk+1].environment.sentPackets, config);
+            } else {
+
+                assert SentDemarshallable(db[kk+1].environment.sentPackets, config);
+            }
+
+            assert mapdomain(db[kk].servers) == mapdomain(db[kk+1].servers);
+
+
+            k := k + 1;
+        }
+
+    }
+  
+
+    lemma RefinementProof(config:ConcreteConfiguration, db:seq<DS_State>) returns (sb:seq<ServiceState>)
+    /*
+        requires |db| > 0
+        requires DS_Init(db[0], config)
+        requires forall i {:trigger DS_Next(db[i], db[i+1])} :: 0 <= i < |db| - 1 ==> DS_Next(db[i], db[i+1]);
+        ensures  |db| == |sb|
+        ensures  Service_Init(sb[0], Collections__Maps2_s.mapdomain(db[0].servers))
+        ensures  forall i {:trigger Service_Next(sb[i], sb[i+1])} :: 0 <= i < |sb| - 1 ==> sb[i] == sb[i+1] || Service_Next(sb[i], sb[i+1])
+        ensures  forall i :: 0 <= i < |db| ==> Service_Correspondence(db[i].environment.sentPackets, sb[i])
+    */
+    {
+
+        var lb := [Construct_LS_State(db[0])];
+        InitTransfer(db[0], config);
+        assert LS_Init(lb[0], config);
+
+        var k := 1;
+        while (k < |db|)
+        invariant 1 <= k <= |db|
+        invariant |lb| == k
+        invariant LS_Init(lb[0], config)
+        invariant forall i :: 0 <= i < k - 1 ==> LS_Next(lb[i], lb[i+1]) || lb[i] == lb[i+1]
+        invariant forall i :: 0 <= i < k ==> lb[i] == Construct_LS_State(db[i])
+        {
+            var servers := ConstructServers(db[k].servers);
+            var lenv := ConstructLEnv(db[k].environment);
+            var kk := k-1;
+            lb := lb + [Construct_LS_State(db[k])];
+            DS_Next_Implies_LS_Next(db[kk], db[kk+1]);
+            assert lb[kk] == Construct_LS_State(db[kk]);
+            assert LS_Next(lb[kk], lb[kk+1]);
+            k := k + 1;
+        }
+
+        sb := LockProof.RefinementProof(config, lb);
+        assert mapdomain(db[0].servers) == MapSeqToSet(config, x=>x);
+        assert mapdomain(db[0].servers) == sb[0].hosts;
+        assert Service_Init(sb[0], Collections__Maps2_s.mapdomain(db[0].servers));
+
+        Valid_Db_Implies_Demarshallable(db, config);
+
+        forall i |
+               0 <= i < |db|
+        ensures Service_Correspondence(db[i].environment.sentPackets, sb[i])
+        {
+            assert lb[i] == Construct_LS_State(db[i]);
+            assert Protocol_Service_Correspondence(lb[i].environment.sentPackets, sb[i]);
+            Valid_Db_Implies_Demarshallable(db, config);
+            assert forall x :: x in sb[i].hosts <==> x in lb[0].servers;
+            assert forall x :: x in config <==> x in sb[i].hosts;
+            ServiceCorrespondenceTransfer(db[i], sb[i]);
+        }
+    }
+
+}
